instructions/binary_search_riscv64/a14.v
@@ -13,7 +13,7 @@ Definition a14 : isla_trace :=
   Smt (DeclareConst 0%Z (Ty_BitVec 64%N)) Mk_annot :t:
   Assume (AExp_Binop (Eq) (AExp_Unop (Extract 2%N 2%N) (AExp_Val (AVal_Var "misa" [Field "bits"]) Mk_annot) Mk_annot) (AExp_Val (AVal_Bits [BV{1%N} 0x1%Z]) Mk_annot) Mk_annot) Mk_annot :t:
   Smt (DeclareConst 1%Z (Ty_BitVec 64%N)) Mk_annot :t:
-  Assume (AExp_Binop (Eq) (AExp_Unop (Extract 17%N 17%N) (AExp_Val (AVal_Var "mstatus" [Field "bits"]) Mk_annot) Mk_annot) (AExp_Val (AVal_Bits [BV{1%N} 0x0%Z]) Mk_annot) Mk_annot) Mk_annot :t:
+  Assume (AExp_Binop (Eq) (AExp_Manyop (Bvmanyarith Bvand) [AExp_Val (AVal_Var "mstatus" [Field "bits"]) Mk_annot; AExp_Val (AVal_Bits [BV{64%N} 0x20000%Z]) Mk_annot] Mk_annot) (AExp_Val (AVal_Bits [BV{64%N} 0x0%Z]) Mk_annot) Mk_annot) Mk_annot :t:
   Smt (DeclareConst 6%Z (Ty_Enum (Mk_enum_id 3%nat))) Mk_annot :t:
   Assume (AExp_Binop (Eq) (AExp_Val (AVal_Var "cur_privilege" []) Mk_annot) (AExp_Val (AVal_Var "Machine" []) Mk_annot) Mk_annot) Mk_annot :t:
   Smt (DeclareConst 7%Z (Ty_BitVec 64%N)) Mk_annot :t:
